mutable_typed_shared_data: Put global invariant inside seal predicate

theories/examples/mutable_typed_shared_data/invariants.v
@@ -2,58 +2,61 @@ From iris.proofmode Require Import proofmode.
 From cap_machine Require Import fundamental logrel macros macros_helpers proofmode rules register_tactics.
 From cap_machine.examples Require Import arch_sealing.
 
-(* This section defines more general definitions and clearer explanations than `arch_sealing`. *)
+(* This section redefines useful definitions from `arch_sealing` along with further explanations. *)
 Section invariants.
   Context {Σ:gFunctors} {memg:memG Σ} {regg:regG Σ} {sealsg: sealStoreG Σ}
           {nainv: logrel_na_invs Σ} `{MP: MachineParameters}.
+
+  (*  *)
+  (* Note: *)
+  Definition seal_pred τ Φ {Hpers : ∀ w, Persistent (Φ w)} := seal_pred τ Φ.
+
+  (* `seal_state` is the combination of `seal_pred` and a specific invariant. *)
+  (* This invariant pin `WSealRange` in memory to retrieve an access to it. *)
+  (* > In our case, `WSealRange` is already pinned and easily accessible. *)
+  (* For simplicity, this example will only use `seal_pred`. *)
 
   (* Fact that the value `w` has been validly sealed satisfying a `Φ` predicate. *)
   (* This definition is close to `interp_sb` and can be obtained using `interp_valid_sealed`. *)
   Definition valid_sealed w τ Φ := valid_sealed w τ Φ.
 
   (* Something sealed is enough to know that the sealed satisfies a predicate `Φ`. *)
-  (* The predicate `Φ` can be refined to a concrete predicate with `seal_state_valid_sealed_pred_eq`. *)
+  (* The predicate `Φ` can be refined to a concrete predicate with `seal_pred_valid_sealed_eq`. *)
   Definition interp_valid_sealed sb τ := interp_valid_sealed sb τ.
 
-  (* TODO: The τ OType is *NOT* in φ - Is this a problem? *)
-  Definition seal_state ι addr (φ : Addr → iPropI Σ) τ Φ {Hpers : ∀ w, Persistent (Φ w)} :=
-    (na_inv logrel_nais ι (φ addr) ∗ seal_pred τ Φ)%I.
-
   (* Concludes that `Φ` ≡ `Φ'` if `seal_state` and `valid_sealed` have the same `τ` OType. *)
-  Definition seal_state_valid_sealed_pred_eq ι addr τ w Φ Φ' {Hpers : ∀ w, Persistent (Φ w)} :=
-    sealLL_valid_sealed_pred_eq ι addr τ w Φ Φ'.
+  (* Note: This is a more-generic version of `sealLL_valid_sealed_pred_eq` *)
+  Lemma seal_pred_valid_sealed_eq τ w Φ Φ' {Hpers : ∀ w, Persistent (Φ w)} :
+    seal_store.seal_pred τ Φ -∗ valid_sealed w τ Φ' -∗ (∀ w, ▷ (Φ w ≡ Φ' w)).
+  Proof.
+    iIntros "Hsp Hvs".
+    iDestruct "Hvs" as (sb) "(_ & _ & Hsp' & _)".
+    iApply (seal_pred_agree with "Hsp Hsp'").
+  Qed.
 
 End invariants.
 
-(* This section refines the definitions specifically for [load_int] and [store_int]. *)
 Section invariants_int.
   Context {Σ:gFunctors} {memg:memG Σ} {regg:regG Σ} {sealsg: sealStoreG Σ}
           {nainv: logrel_na_invs Σ} `{MP: MachineParameters}.
 
-  Notation "a ↪ₐ w" := (mapsto (L := Addr) (V := Word) a DfracDiscarded w) (at level 20) : bi_scope.
+  Definition seal_intN : namespace := nroot .@ "seal".
 
-  Definition sealN : namespace := nroot .@ "seal".
-
-  Definition int_sealed: Word → iProp Σ :=
-    (λ w, (∃ a_cap w', ⌜w = WCap RW a_cap (a_cap ^+ 1)%a a_cap⌝ ∗ a_cap ↪ₐ w' ∗ ⌜is_z w'⌝)%I).
-
-  Instance int_sealed_timeless w : Timeless (int_sealed w).
-  Proof. apply _. Qed.
+  Definition int_sealed : Word → iProp Σ :=
+    (λ w, (∃ a_cap, ⌜w = WCap RW a_cap (a_cap ^+ 1)%a a_cap⌝
+                         ∗ na_inv logrel_nais seal_intN (∃ w, a_cap ↦ₐ w ∗ ⌜is_z w⌝))%I).
 
   Instance int_sealed_persistent w : Persistent (int_sealed w).
   Proof. apply _. Qed.
 
-  (* TODO: ⌜is_z w⌝ should not be there *)
-  Definition seal_state_int ι addr τ: iProp Σ :=
-    seal_state ι addr (λ addr, ∃ w, addr ↦ₐ w ∗ ⌜is_z w⌝)%I τ int_sealed.
-
+  (* Integer-specific redefinitions *)
+  Definition seal_pred_int τ := seal_pred τ int_sealed.
   Definition valid_sealed_int w τ := valid_sealed w τ int_sealed.
 
-  Lemma seal_state_int_valid_sealed_pred_eq ι addr τ w Φ :
-    seal_state_int ι addr τ -∗ valid_sealed w τ Φ -∗  (∀ w, ▷ (int_sealed w ≡ Φ w)).
+  Lemma seal_state_int_valid_sealed_pred_eq τ w Φ :
+    seal_pred τ int_sealed -∗ valid_sealed w τ Φ -∗  (∀ w, ▷ (int_sealed w ≡ Φ w)).
   Proof.
-    iIntros "HsealLL Hvs".
-    iDestruct "HsealLL" as "[_ Hsp]".
+    iIntros "Hsp Hvs".
     iDestruct "Hvs" as (sb) "(_ & _ & Hsp' & _)".
     iApply (seal_pred_agree with "Hsp Hsp'").
   Qed.
